bench/sources/rename.c
@@ -1,0 +1,101 @@
+#include <stdio.h>
+#include <errno.h>
+#include <fcntl.h>
+#include <stdlib.h>
+#include <unistd.h>
+#include <string.h>
+#include <stdint.h>
+#include <sys/stat.h>
+#include <sys/types.h>
+#include <sys/time.h>
+
+#define N 1000
+#define FILESIZE 100
+#define NAMESIZE 100
+
+static char newname[NAMESIZE];
+static char oldname[NAMESIZE];
+static char buf[FILESIZE]; 
+static char *dir;
+
+void printstats(int reset)
+{
+  int fd;
+  int r;
+
+  sprintf(oldname, "%s/stats", dir);
+  if((fd = open(oldname, O_RDONLY)) < 0) {
+    return;
+  }
+
+  bzero(buf, FILESIZE);
+
+  if ((r = read(fd, buf, FILESIZE)) < 0) {
+    perror("read");
+    exit(1);
+  }
+
+  if (!reset)
+    fprintf(stdout, "=== FS Stats ===\n%s========\n", buf);
+
+  if ((r = close(fd)) < 0) {
+    perror("close");
+  }
+}
+
+static uint64_t
+usec_now()
+{
+  struct timeval tv;
+
+  gettimeofday(&tv, NULL);
+
+  uint64_t res = tv.tv_sec;
+  res *= 1000000;
+  res += tv.tv_usec;
+  return res;
+}
+
+int main(int argc, char *argv[])
+{
+  int i;
+  int r;
+  int fd;
+  uint64_t start, end;
+
+  if (argc != 2) {
+    printf("Usage: %s basedir\n", argv[0]);
+    exit(-1);
+  }
+  
+  dir = argv[1];
+  sprintf(buf, "%s/d", argv[1]);
+  if (mkdir(buf,  S_IRWXU) < 0) {
+    printf("%s: mkdir %s failed %s\n", argv[0], buf, strerror(errno));
+    exit(1);
+  }
+  printstats(1);
+  start = usec_now();
+  sprintf(oldname, "%s/d/f%d", argv[1], 0);
+  sprintf(newname, "%s/d/f%d", argv[1], 1);
+  if((fd = open(oldname, O_RDWR | O_CREAT | O_TRUNC, S_IRWXU)) < 0) {
+    printf("%s: create %s failed %s\n", argv[0], oldname, strerror(errno));
+    exit(1);
+  }
+  close(fd);  
+  for (i = 1; ; i++) {
+    if((fd = open(newname, O_RDWR | O_CREAT | O_TRUNC, S_IRWXU)) < 0) {
+      printf("%s: create %s failed %s\n", argv[0], newname, strerror(errno));
+      exit(1);
+    }
+    close(fd);  
+    rename(newname, oldname);
+    end = usec_now();
+    if (end - start > 1000000)
+      break;
+  }
+
+  printf("DATA: %d %ld\n", i, end-start);
+
+  printstats(0);
+}
