src/Extraction/Interpreter/ConFs.hs
@@ -25,10 +25,18 @@ import System.Posix.User
 import qualified BaseTypes
 import qualified File
 import qualified Interpreter
-
+import Data.Serialize
+import Directory
+import qualified Data.Text
+import Data.Text.Encoding (encodeUtf8, decodeUtf8)
+import qualified Helpers
+import qualified Data.ByteString.Char8 as BSC8
 
 -- Handle type for open files; we will use the inode number
 type HT = BaseTypes.Coq_addr
+
+blocksize :: Int
+blocksize = BaseTypes.block_size `div` 8
 
 verboseFuse :: Bool
 verboseFuse = False
@@ -59,54 +67,229 @@ main = do
     fn:rest -> run_fuse fn rest
     _ -> putStrLn $ "Usage: fuse disk -f /tmp/ft"
 
+
 run_fuse :: String -> [String] -> IO ()
 run_fuse disk_fn fuse_args = do
-  fileExists <- System.Directory.doesFileExist disk_fn
-  {- 
-    ds <- case disk_fn of
-    "/tmp/crashlog.img" -> init_disk_crashlog disk_fn
-    _ -> init_disk disk_fn
-  -}
-  _ <- writeIORef Interpreter.txnList []
-  _ <- writeIORef Interpreter.cache Data.Map.empty
-  _ <- writeIORef Interpreter.cipherMap Data.Map.empty
-  s <- if fileExists
-  then
-    do
-      putStrLn $ "Recovering file system"
-      File.recover
-  else
-    do
-      putStrLn $ "Initializing file system"
-      fs <- openBinaryFile disk_fn ReadWriteMode
-      _ <- writeIORef Interpreter.fsImage fs
-      File.init
   putStrLn $ "Starting file system."
-  fuseRun "confs" fuse_args (confsFSOps getFuseContext) defaultExceptionHandler
+  fuseRun "confs" fuse_args (confsFSOps disk_fn getFuseContext) defaultExceptionHandler
+
+fileStat :: FuseContext -> FileStat
+fileStat ctx = FileStat { statEntryType = RegularFile
+, statFileMode = foldr1 unionFileModes
+                    [ ownerReadMode, ownerWriteMode, ownerExecuteMode
+                    , groupReadMode, groupWriteMode, groupExecuteMode
+                    , otherReadMode, otherWriteMode, otherExecuteMode
+                    ]
+, statLinkCount = 1
+, statFileOwner = fuseCtxUserID ctx
+, statFileGroup = fuseCtxGroupID ctx
+, statSpecialDeviceID = 0
+, statFileSize = 0
+, statBlocks = 1
+, statAccessTime = 0
+, statModificationTime = 0
+, statStatusChangeTime = 0
+}
+
+dirStat :: FuseContext -> FileStat
+dirStat ctx = FileStat { statEntryType = Directory
+  , statFileMode = foldr1 unionFileModes
+                      [ ownerReadMode, ownerWriteMode, ownerExecuteMode
+                      , groupReadMode, groupExecuteMode
+                      , otherReadMode, otherExecuteMode
+                      ]
+  , statLinkCount = 2
+  , statFileOwner = fuseCtxUserID ctx
+  , statFileGroup = fuseCtxGroupID ctx
+  , statSpecialDeviceID = 0
+  , statFileSize = 4096
+  , statBlocks = 1
+  , statAccessTime = 0
+  , statModificationTime = 0
+  , statStatusChangeTime = 0
+  }
 
 -- See the HFuse API docs at:
 -- https://hackage.haskell.org/package/HFuse-0.2.1/docs/System-Fuse.html
-confsFSOps :: IO FuseContext -> FuseOperations HT
-confsFSOps getctx  = defaultFuseOps
-  { fuseOpen = confsOpen
-  , fuseRead = confsRead
-  , fuseWrite = confsWrite
-  , fuseRemoveLink = confsUnlink
-  , fuseSetOwnerAndGroup = confsChown
+confsFSOps :: String -> IO FuseContext -> FuseOperations HT
+confsFSOps disk_fn getctx  = defaultFuseOps
+  { fuseGetFileStat = confsGetFileStat getctx
+  , fuseReadSymbolicLink = \ path -> do
+    print "--confsReadSymbolicLink--"
+    print path
+    return (Left eIO)
   , fuseCreateDevice = confsCreateDevice
   , fuseCreateDirectory = confsCreateDirectory
+  , fuseRemoveLink = confsUnlink
+  , fuseRemoveDirectory = confsRemoveDirectory
+  , fuseCreateSymbolicLink = \ _ _ -> return eOK
+  , fuseRename = confsRename
+  , fuseCreateLink = \ _ _ -> return eOK
+  , fuseSetFileMode = \ _ _ -> return eOK
+  , fuseSetOwnerAndGroup = confsChown
+  , fuseSetFileSize = \ _ _ -> return eOK
+  , fuseSetFileTimes = \ _ _ _ -> return eOK
+  , fuseOpen = confsOpen
+  , fuseRead = confsRead
+  , fuseWrite = confsWrite
+  , fuseGetFileSystemStats = confsGetFileSystemStats
+  , fuseFlush = \ _ _ -> return eOK
+  , fuseRelease = \ _ _ -> return ()
+  , fuseSynchronizeFile = \ _ _ -> return eOK
   , fuseOpenDirectory = confsOpenDirectory
+  , fuseReadDirectory = confsReadDirectory getctx
+  , fuseReleaseDirectory = \ _ -> return eOK
+  , fuseSynchronizeDirectory = \ _ _ -> return eOK
+  , fuseAccess = \ _ _ -> return eOK
+  , fuseInit = confsInit disk_fn
+  , fuseDestroy = confsDestroy
   }
 
--- needed for tests
+confsDestroy :: IO ()
+confsDestroy = do
+  stats <- Interpreter.diskClose
+  Interpreter.printStats stats
+
+confsReadDirectory :: IO FuseContext -> FilePath -> IO (Either Errno [(FilePath, FileStat)])  
+confsReadDirectory getctx path = do
+  let path_list = (splitDirectories path)
+  r <- onDirMap (isValidDirPath path_list)
+  if r then do
+    msd <- onDirMap (getSubdirs (last path_list))
+    case msd of
+      Just sd -> do
+        ctx <- getctx
+        return (Right (map (\s -> (s, dirStat ctx)) sd))
+      Nothing -> return (Left eIO)
+  else
+    return (Left eIO)
+
+confsGetFileStat :: IO FuseContext -> FilePath -> IO (Either Errno FileStat)
+confsGetFileStat getctx path 
+    | (last (splitDirectories path) == "stats") || 
+      (last (splitDirectories path) == "sync") = do
+        ctx <- getctx
+        return (Right (fileStat ctx))
+    | otherwise = do
+    -- print "--confsGetFileStat--"
+    -- print path
+    let path_list = (splitDirectories path)
+    r <- onDirMap (isValidDirPath path_list)
+    if r then do
+      ctx <- getctx
+      return (Right (dirStat ctx))
+    else do
+      r <- onDirMap (isValidFilePath path_list)
+      if r then do
+        ctx <- getctx
+        return (Right (fileStat ctx))
+      else
+        return (Left eNOENT)
+
+confsRename :: FilePath -> FilePath -> IO Errno
+confsRename src dst = do
+  --print "--confsRename--"
+  --print src
+  --print dst
+  let src_path_list = (splitDirectories src)
+  let dst_path_list = (splitDirectories dst)
+  r <- onDirMap (isValidPath src_path_list)
+  if r then do
+    r <- onDirMap (isValidPath dst_path_list)
+    if r then do
+          r <- modifyDirMap (Directory.rename src_path_list dst_path_list)
+          persistDirMap
+          return r
+    else 
+      return eIO
+  else
+    return eIO
+
+confsRemoveDirectory :: FilePath -> IO Errno
+confsRemoveDirectory path = do
+  --print "--confsRemoveDirectory--"
+  --print path
+  let path_list = (splitDirectories path)
+  modifyDirMap (removeDir path_list)
+
+confsGetFileSystemStats :: String -> IO (Either Errno FileSystemStats)
+confsGetFileSystemStats path = do
+  --print "--confsGetFileSystemStats--"
+  --print path
+  return $ Right $ FileSystemStats
+    { fsStatBlockSize = 4096
+    , fsStatBlockCount = 2 * 8 * 4096
+    , fsStatBlocksFree = 2 * 8 * 4096
+    , fsStatBlocksAvailable = 2 * 8 * 4096
+    , fsStatFileCount = 8 * 4096
+    , fsStatFilesFree = 2 * 8 * 4096
+    , fsStatMaxNameLength = 128
+    }
+
+confsInit:: String -> IO ()
+confsInit disk_fn = do
+  -- print "--confsInit--"
+  -- print disk_fn
+  _ <- writeIORef Interpreter.txnList []
+  _ <- writeIORef Interpreter.cache Data.Map.empty
+  _ <- writeIORef Interpreter.cipherMap Data.Map.empty
+  fileExists <- System.Directory.doesFileExist disk_fn
+  fs <- openBinaryFile disk_fn ReadWriteMode
+  writeIORef Interpreter.fsImage fs
+  if fileExists then do
+    putStrLn $ "Recovering file system"
+    File.recover
+    recoverDirMap
+  else do
+    putStrLn $ "Initializing file system"
+    File.init
+    initializeDirMap
+
 confsCreateDevice :: FilePath -> EntryType -> FileMode -> DeviceID -> IO Errno
-confsCreateDevice _ _ _ _ = return eOK
+confsCreateDevice path entryType _ _ = do
+  -- print "--confsCreateDevice--"
+  -- print path
+  -- print entryType
+  case entryType of
+    RegularFile -> do
+      let path_list = (splitDirectories path)
+      --print "Path List:"
+      --print path_list
+      r <- onDirMap (isValidDirPath (take (length path_list - 1) path_list))
+      if r then do
+        r <- onDirMap (Data.Map.notMember (last path_list))
+        if r then do
+          uid <- getEffectiveUserID
+          minum <- File.create uid
+          case minum of
+            Just inum -> modifyDirMap (addFile path_list inum)
+            Nothing -> return eNOSPC
+        else
+          return eEXIST
+      else
+        return eNOTDIR
+    _ -> return eIO
 
 confsCreateDirectory :: FilePath -> FileMode -> IO Errno
-confsCreateDirectory _ _ = return eOK
+confsCreateDirectory path _ = do
+  --print "--confsCreateDirectory--"
+  --print path
+  let path_list = (splitDirectories path)
+  modifyDirMap (addDir path_list)
 
 confsOpenDirectory :: FilePath -> IO Errno
-confsOpenDirectory _ = return eOK
+confsOpenDirectory path 
+  | (last (splitDirectories path) == "stats") || 
+    (last (splitDirectories path) == "sync") = return eOK
+  | otherwise = do
+    --print "--confsOpenDirectory--"
+    --print path
+    let path_list = (splitDirectories path)
+    r <- onDirMap (isValidDirPath path_list)
+    if r then
+      return eOK
+    else
+      return eIO
   
 writeSubsets' :: [[(Integer, a)]] -> [[(Integer, a)]]
 writeSubsets' [] = [[]]
@@ -121,39 +304,57 @@ writeSubsets writes = writeSubsets' addrWrites
     addrWrites = Data.List.groupBy sameaddr writes
     sameaddr (x, _) (y, _) = (x == y)
 
--- I will use this as create, ignoring path, modes etc.
+-- modes etc.
 confsOpen :: FilePath -> OpenMode -> OpenFileFlags -> IO (Either Errno HT)
-confsOpen _ _ _ = do
-  uid <- System.Posix.User.getEffectiveUserID
-  r <- File.create uid
-  case r of
-    Nothing -> return $ Left $ eIO
-    Just inum -> return $ Right inum
+confsOpen path _ _ 
+  | (last (splitDirectories path) == "stats") || 
+    (last (splitDirectories path) == "sync") = return $ Right 0
+  | otherwise = do
+    --print "--confsOpen--"
+    --print path
+    let path_list = (splitDirectories path)
+    r <- onDirMap (isValidFilePath path_list)
+    if r then do
+      minum <- onDirMap (getInum (last path_list))
+      case minum of
+        Just inum -> return (Right inum)
+        Nothing -> return (Left eIO)
+    else
+      return (Left eIO)
 
--- use path as string representation of handle
 confsUnlink :: FilePath -> IO Errno
 confsUnlink path = do
-  case readMaybe path of
-    Just i -> do
-      r <- File.delete i
-      case r of
-        Just _ -> return eOK
-        Nothing -> return eIO
-    Nothing -> return eIO
+  --print "--confsUnlink--"
+  --print path
+  let path_list = (splitDirectories path)
+  r <- onDirMap (isValidFilePath path_list)
+  if r then do
+    minum <- onDirMap (getInum (last path_list))
+    case minum of
+      Just inum -> do 
+        r <- File.delete inum
+        case r of
+          Just _ -> modifyDirMap (removeFile path_list)
+          Nothing -> return eIO
+      Nothing -> return eIO
+  else
+    return eIO
 
--- use file path as string rep of handle.
 confsChown :: FilePath -> UserID -> GroupID -> IO Errno
 confsChown path uid _  = do
-  case readMaybe path of
-    Just i -> do
-      r <- File.change_owner i (fromIntegral (toInteger uid))
+  --print "--confsChown--"
+  --print path
+  r <- onDirMap (isValidFilePath (splitDirectories path))
+  if r then do
+    minum <- onDirMap (getInum (takeFileName path))
+    case minum of
+      Just inum -> do 
+      r <- File.change_owner inum (fromIntegral (toInteger uid))
       case r of
         Just _ -> return eOK
         Nothing -> return eIO
-    Nothing -> return eIO
-
-blocksize :: Int
-blocksize = BaseTypes.block_size `div` 8
+  else
+    return eIO
 
 data BlockRange =
   BR !Int !Int !Int   -- blocknumber, offset-in-block, count-from-offset
@@ -171,17 +372,26 @@ compute_ranges off count =
   compute_ranges_int (fromIntegral off) (fromIntegral count)
 
 confsRead :: FilePath -> HT -> ByteCount -> FileOffset -> IO (Either Errno BS.ByteString)
-confsRead _ inum byteCount offset = do
-  pieces <- mapM read_piece $ compute_ranges offset byteCount
-  return $ Right $ BS.concat pieces
-  where
-    read_piece (BR blk off count) = do
-      ok_buf <- File.read inum blk
-      case ok_buf of
-        Just buf ->
-          return $ BS.take count $ BS.drop off $ buf
-        Nothing ->
-          error "Read ERROR"
+confsRead path inum byteCount offset 
+  | last (splitDirectories path) == "stats" = do
+    Interpreter.Stats r w s <- Interpreter.getStats
+    Interpreter.clearStats
+    let bs = BSC8.pack ("Reads:  " ++ (show r) ++ "\n" ++ "Writes: " ++ (show w) ++ "\n" ++ "Syncs:  " ++ (show s) ++ "\n")
+    print bs
+    return $ (Right bs)
+  | otherwise = do
+    print "--confsRead--"
+    print path
+    pieces <- mapM read_piece $ compute_ranges offset byteCount
+    return $ Right $ BS.concat pieces
+    where
+      read_piece (BR blk off count) = do
+        ok_buf <- File.read inum blk
+        case ok_buf of
+          Just buf ->
+            return $ BS.take count $ BS.drop off $ buf
+          Nothing ->
+            error "Read ERROR"
 
 compute_range_pieces :: FileOffset -> BS.ByteString -> [(BlockRange, BS.ByteString)]
 compute_range_pieces off buf = zip ranges pieces
@@ -197,7 +407,9 @@ data WriteState =
 
 -- This should automatically extend if it passes file length
 confsWrite :: FilePath -> HT -> BS.ByteString -> FileOffset -> IO (Either Errno ByteCount)
-confsWrite _ inum bs offset = do
+confsWrite path inum bs offset = do
+  --print "--confsWrite--"
+  --print path
   mlen <- File.get_file_size inum
   case mlen of
     Just len -> do
@@ -231,7 +443,7 @@ confsWrite _ inum bs offset = do
                 Nothing -> return (WriteErr c)
             Nothing -> return (WriteErr c)
       else do
-        r <- File.extend inum piece_bs
+        r <- File.extend inum (BS.append piece_bs (BS.replicate (blocksize - BS.length piece_bs) 0))
         case r of
           Just _ -> return (WriteOK (c + (fromIntegral cnt)))
           Nothing -> return (WriteErr c)
