src/Extraction/Interpreter/Directory.hs
@@ -1,0 +1,247 @@
+module Directory where
+
+import Prelude
+import Data.Map
+import Data.IORef
+import BaseTypes
+import GHC.IO.Unsafe
+import qualified Interpreter
+import Data.Serialize
+import Foreign.C.Error
+import Data.Maybe
+import qualified Data.List as L
+import Data.String
+import qualified Helpers
+import qualified Data.ByteString as BS
+{-
+Haskell implemented directories all names should be unique
+-}
+dirMapAddr :: Int
+dirMapAddr = 0
+
+-- This is a map from directory names to list of files/dirs under it.
+-- if it is a file, then second field contains its inode number, which should be used as the file descriptor
+dirMap :: IORef (Map String (Either [String] Coq_addr))
+{-# NOINLINE dirMap #-}
+dirMap = unsafePerformIO (newIORef empty)
+
+initializeDirMap :: IO ()
+initializeDirMap = do
+  writeIORef dirMap (insert "/" (Left []) empty)
+  persistDirMap
+
+recoverDirMap :: IO ()
+recoverDirMap = do
+  dirBlock <- Interpreter.diskRead dirMapAddr
+  let edm = (decode dirBlock)
+  --print "--Recovering dirMap"
+  --print edm
+  case edm of
+    Left e -> print e
+    Right dm -> writeIORef dirMap dm
+
+persistDirMap :: IO ()
+persistDirMap = do
+  dm <- readIORef dirMap
+  --print "--Persisting dirMap"
+  --print dm
+  let dmBlock = Helpers.setToBlockSize (div block_size 8) (encode dm) 
+  Interpreter.diskWrite dirMapAddr dmBlock
+  Interpreter.diskSync
+
+
+getInum :: String -> Map String (Either [String] Coq_addr) -> Maybe Coq_addr
+getInum fn dm =
+  case Data.Map.lookup fn dm of
+    Nothing -> Nothing
+    Just e ->
+      case e of
+        Right i -> Just i
+        Left sl -> Nothing
+
+getSubdirs :: String -> Map String (Either [String] Coq_addr) -> Maybe [String]
+getSubdirs fn dm =
+  case Data.Map.lookup fn dm of
+    Nothing -> Nothing
+    Just e ->
+      case e of
+        Right _ -> Nothing
+        Left sl -> Just sl
+
+isDir ::  String -> Map String (Either [String] Coq_addr) -> Bool
+isDir d dm = isJust (getSubdirs d dm)
+
+isSubdir ::  String -> String -> Map String (Either [String] Coq_addr) -> Bool
+isSubdir parent child dm =
+  case Data.Map.lookup parent dm of
+    Nothing -> False
+    Just e ->
+      case e of
+        Right _ -> False
+        Left sl -> elem child sl
+
+isFile :: String -> Map String (Either [String] Coq_addr) -> Bool
+isFile d dm = isJust (getInum d dm)
+
+isValidPath :: [String] -> Map String (Either [String] Coq_addr) -> Bool
+isValidPath [c] dm = isDir c dm || isFile c dm
+isValidPath (p : c : rest) dm = isSubdir p c dm && isValidPath (c:rest) dm
+
+isValidDirPath :: [String] -> Map String (Either [String] Coq_addr) -> Bool
+isValidDirPath [c] dm = isDir c dm
+isValidDirPath (p : c : rest) dm = isSubdir p c dm && isValidDirPath (c:rest) dm
+
+isValidFilePath :: [String] -> Map String (Either [String] Coq_addr) -> Bool
+isValidFilePath [c] dm = isFile c dm
+isValidFilePath (p : c : rest) dm = isSubdir p c dm && isValidFilePath (c:rest) dm
+
+
+{- Modifiers -}
+rename_with_parent :: String -> String -> String -> String -> Map String (Either [String] Coq_addr) -> (Map String (Either [String] Coq_addr) , Errno)
+rename_with_parent sp sc dp dc dm =
+      case Data.Map.lookup sp dm of
+      Nothing -> (dm, eIO)
+      Just spd ->
+        case spd of
+        Right _ -> (dm, eIO)
+        Left sl -> 
+          case Data.Map.lookup dp dm of
+          Nothing -> (dm, eIO)
+          Just dpd ->
+            case dpd of
+            Right _ -> (dm, eIO)
+            Left dl -> 
+              case Data.Map.lookup sc dm of
+              Nothing -> (dm, eIO)
+              Just scf ->
+                (Data.Map.insert dc scf 
+                (Data.Map.insert dp (Left (dc:dl)) 
+                (Data.Map.insert sp (Left (L.delete sc sl))
+                (Data.Map.delete sc dm))), eOK)
+
+rename_single :: String -> String -> Map String (Either [String] Coq_addr) -> (Map String (Either [String] Coq_addr) , Errno)
+rename_single sc dc dm =
+    case Data.Map.lookup sc dm of
+    Nothing -> (dm, eIO)
+    Just scf ->
+      (Data.Map.insert dc scf (Data.Map.delete sc dm), eOK)
+
+rename :: [String] -> [String] -> Map String (Either [String] Coq_addr) -> (Map String (Either [String] Coq_addr) , Errno)
+rename [sc] [dc] dm = rename_single sc dc dm
+rename [sp, sc] [dp, dc] dm = rename_with_parent sp sc dp dc dm
+rename (sp : sc : srest) (dp : dc : drest) dm = 
+  let (dm', e) = rename (sc:srest) (dc:drest) dm in
+    case e of
+      eOK -> rename_with_parent sp sc dp dc dm'
+      _ -> (dm, e)
+    
+
+removeDir :: [String] -> Map String (Either [String] Coq_addr) -> (Map String (Either [String] Coq_addr) , Errno)
+removeDir [c] dm = (Data.Map.delete c dm, eOK)
+removeDir [p, c] dm = 
+  case Data.Map.lookup p dm of
+    Nothing -> (dm, eIO)
+    Just dpd ->
+      case dpd of
+        Right _ -> (dm, eIO)
+        Left pl ->
+          case Data.Map.lookup c dm of
+            Nothing -> (dm, eIO)
+            Just dcd ->
+              case dcd of
+                Right _ -> (dm, eIO)
+                Left cl ->
+                  if cl == [] then
+                    (Data.Map.delete c 
+                    (Data.Map.insert p (Left (L.delete c pl)) dm), eOK)
+                  else
+                    (dm, eIO)
+removeDir (p : c : rest) dm = 
+  if (isSubdir p c dm) then
+    removeDir (c:rest) dm
+  else
+    (dm, eIO)
+
+removeFile :: [String] -> Map String (Either [String] Coq_addr) -> (Map String (Either [String] Coq_addr) , Errno)
+removeFile [p, c] dm = 
+  case Data.Map.lookup p dm of
+    Nothing -> (dm, eIO)
+    Just dpd ->
+      case dpd of
+        Right _ -> (dm, eIO)
+        Left pl ->
+            if (isFile c dm) then 
+              (Data.Map.delete c (Data.Map.insert p (Left (L.delete c pl)) dm), eOK)
+            else
+              (dm, eIO)
+
+removeFile (p : c : rest) dm = 
+  if (isSubdir p c dm) then
+    removeFile (c:rest) dm
+  else
+    (dm, eIO)
+
+addDir :: [String] -> Map String (Either [String] Coq_addr) -> (Map String (Either [String] Coq_addr) , Errno)
+addDir [c] dm = 
+  if (isFile c dm) || (isDir c dm) then 
+    (dm, eIO)
+  else
+    (Data.Map.insert c (Left []) dm, eOK)
+addDir [p, c] dm = 
+      case Data.Map.lookup p dm of
+        Nothing -> (dm, eIO)
+        Just dpd ->
+          case dpd of
+            Right _ -> (dm, eIO)
+            Left pl ->
+                if (isFile c dm) || (isDir c dm) then 
+                  (dm, eIO)
+                else
+                  (Data.Map.insert c (Left []) (Data.Map.insert p (Left (c : pl)) dm), eOK)
+                  
+    
+addDir (p : c : rest) dm = 
+  if (isSubdir p c dm) then
+    addDir (c:rest) dm
+  else
+    (dm, eIO)
+
+addFile :: [String] -> Coq_addr -> Map String (Either [String] Coq_addr) -> (Map String (Either [String] Coq_addr) , Errno)
+addFile [c] inum dm = 
+  if (isFile c dm) || (isDir c dm) then 
+    (dm, eIO)
+  else
+    (Data.Map.insert c (Right inum) dm, eOK)
+
+addFile [p, c] inum dm = 
+  case Data.Map.lookup p dm of
+    Nothing -> (dm, eIO)
+    Just dpd ->
+      case dpd of
+        Right _ -> (dm, eIO)
+        Left pl ->
+            if (isFile c dm) || (isDir c dm) then 
+              (dm, eIO)
+            else
+              (Data.Map.insert c (Right inum)
+              (Data.Map.insert p (Left (c:pl)) dm), eOK)
+              
+        
+addFile (p : c : rest) inum dm = 
+  if (isSubdir p c dm) then
+    addFile (c:rest) inum dm
+  else
+    (dm, eIO)
+
+onDirMap :: (Map String (Either [String] Coq_addr) -> a) -> IO a
+onDirMap f = do
+  dm <- readIORef dirMap
+  return (f dm)
+
+modifyDirMap :: (Map String (Either [String] Coq_addr) -> (Map String (Either [String] Coq_addr) , a)) -> IO a
+modifyDirMap f = do 
+  dm <- readIORef dirMap
+  let (newMap, ret) = f dm
+  writeIORef dirMap newMap
+  --persistDirMap
+  return ret
