src/Extraction/Interpreter/mkfs.hs
@@ -1,17 +1,31 @@
 module Main where
 
 import qualified File
+import qualified Interpreter
+import qualified Data.Map
+import Directory
+import qualified System.Directory
 import System.Environment
+import Data.IORef
+import System.IO
 
 main :: IO ()
 main = do
   args <- getArgs
   case args of
     [fn] -> do
-      putStrLn $ "Initializing file system"
-      res <- File.init
-      case res of
-        Nothing -> error $ "mkfs failed"
-        Just _ -> putStrLn "Initialization OK!"
+      confsInit fn
     _ -> do
       putStrLn $ "Usage: mkfs diskpath"
+
+confsInit:: String -> IO ()
+confsInit disk_fn = do
+  print "--MKFS--"
+  print disk_fn
+  _ <- writeIORef Interpreter.txnList []
+  _ <- writeIORef Interpreter.cache Data.Map.empty
+  _ <- writeIORef Interpreter.cipherMap Data.Map.empty
+  fs <- openBinaryFile disk_fn ReadWriteMode
+  writeIORef Interpreter.fsImage fs
+  File.init
+  initializeDirMap
