bench/compile-and-run.sh
@@ -1,0 +1,8 @@
+cd ../src/Extraction/
+./compile.sh
+cd ../../bench
+mv ../src/Extraction/extracted/ConFs ./fs/ConFs
+mv ../src/Extraction/extracted/mkfs ./fs/mkfs
+./compile-sources.sh
+./run-all.sh 3
+#sudo ./test.sh ConFs smallfile /dev/sda6 1
