bench/compile-sources.sh
@@ -1,3 +1,5 @@
 gcc -o tests/smallfile sources/smallfile.c
 gcc -o tests/largefile sources/largefile.c
 gcc -o tests/createdelete sources/createdelete.c
+gcc -o tests/rename sources/rename.c
+#gcc -o tests/fsstats sources/fsstats.c
