bench/run-all.sh
@@ -7,16 +7,22 @@ fi
 
 rm -rf results
 mkdir results
-mkdir results/confs
+mkdir results/ConFs
 
 echo "=== Running ConFs Tests ==="
 
 echo "== smallfile =="
-./run_script.sh disk_img smallfile /dev/sda1 $ITER > results/confs/smallfile
+./run_script.sh ConFs smallfile /dev/sdb3 $ITER > results/ConFs/smallfile
 echo "== largefile =="
-./run_script.sh disk_img largefile /dev/sda1 $ITER > results/confs/largefile
+./run_script.sh ConFs largefile /dev/sdb3 $ITER > results/ConFs/largefile
 echo "== createdelete =="
-./run_script.sh disk_img createdelete /dev/sda1 $ITER > results/confs/createdelete
+./run_script.sh ConFs createdelete /dev/sdb3 $ITER > results/ConFs/createdelete
+echo "== rename =="
+./run_script.sh ConFs rename /dev/sdb3 $ITER > results/ConFs/rename
 
 python process-results.py > results.txt
 python process-results-largefile.py >> results.txt
+
+# echo "=== ConFs Stats ===" > stat-results.txt
+# cat results/ConFs/fsstats >> stat-results.txt
+# echo "" >> stat-results.txt
