bounds.v
@@ -1,0 +1,14 @@
+Crash Before
+length o < c1 * 4 + 8
+or
+length o < c2 * 4 + 10
+or
+(length o > c2 * 4 + c3 + 11 /\
+length o <= c2 * 4 + c3 + c1 * 4 + 23)
+or
+length o >= c2 * 4 + 10 /\
+length o <  c2 * 4 + c3 + 16)
+or
+length o >= c2 * 4 + c3 + 16
+
+Crash After
