src/Extraction/compile.sh
@@ -1,6 +1,6 @@
 #! /bin/bash
 
-rm -rf ./extracted
+rm -rf -f ./extracted
 mkdir extracted
 cp ./*.hs ./extracted
 cp ./Interpreter/*.hs ./extracted
@@ -50,5 +50,6 @@ sed -ie '/^module/a import qualified Crypto.Hash.Algorithms' BaseTypes.hs
 sed -ie '/^module/a import Prelude' BaseTypes.hs
 
 # Compile Haskell files 
-ghc ConFs.hs
+ghc -threaded ConFs.hs
+ghc -threaded mkfs.hs
 
